Add TotalMap and PartialMap definitions

semantics/Imp.v
@@ -18,54 +18,164 @@ Definition env := stringmap loc.
 Inductive expr: Type :=
 | Const (n: nat)
 | Addr (x: string)
-| LVal (e: expr)
-with lval: Type :=
 | Deref (e: expr).
 
 Inductive stmt: Type :=
 | Skip
-| Assign (x: string) (e: expr)
-| Alloc (x: string) (mu: string).
+| Assign (x: string) (e: expr).
+(* | Alloc (x: string) (mu: string). *)
 
-Fixpoint eval_expr (mem: mem) (env: env) (expr: expr): option value :=
+Definition eval_expr (mem: mem) (env: env) (expr: expr): value :=
   match expr with
-  | Const n => Some (VInt n)
+  | Const n => VInt n
   | Addr x =>
     match env !! x with
-    | Some l => mem !! l
-    | None => None
+    | Some l => match mem !! l with 
+                | Some v => v
+                | None => VInt 0
+                end
+    | None => VInt 0
     end
-  | LVal e => match eval_expr mem env e with
-              | Some (VLoc l) => mem !! l
-              | _ => None
-              end
-  end.
+  | Deref e => match e with
+    | Addr x => match env !! x with
+                | Some l => match mem !! l with 
+                            | Some v => v
+                            | None => VInt 0
+                            end
+                | None => VInt 0
+                end
+    | _ => VInt 0
+    end
+end.
 
-Definition eval_lval (mem: mem) (env: env) (lval: lval): option value :=
+Definition eval_lval (mem: mem) (env: env) (lval: expr): value :=
   match lval with
   | Deref e => eval_expr mem env e
+  | _ => VInt 0
   end.
 
 Definition def_heap := VInt 0.
 
-Definition eval_stmt (m: mem) (e: env) (s: stmt): option (mem * env) :=
+Definition eval_stmt (m: mem) (e: env) (s: stmt): mem * env :=
   match s with
-  | Skip => Some (m, e)
+  | Skip => (m, e)
   | Assign x expr =>
-    match eval_expr m e expr with
-    | Some v => let m' := map_insert x v m in
-                let e' := map_insert x x e in
-                  Some (m', e')
-    | None => None
-    end
-  | Alloc x mu => 
-                let m' := map_insert x def_heap m in
-                let e' := map_insert x mu e in
-                Some (m', e')
-  end.
+        let v := eval_expr m e expr in
+        let m' := map_insert x v m in
+        let e' := map_insert x x e in
+        (m', e')
+      end.
 
-Theorem eval_stmt_eq: forall (m m': mem) (e e': env) (s: stmt),
+(* Theorem eval_stmt_eq: forall (m m': mem) (e e': env) (s: stmt),
   m = m' /\ e = e' -> eval_stmt m e s = eval_stmt m' e' s.
 Proof.
   intros. destruct H as [Hm He]. rewrite Hm. rewrite He. reflexivity.
-Qed.
+Qed. *)
+
+Definition state := (mem * env)%type.
+
+(* Read and Written sets *)
+Definition locs := stringset.
+Definition vars := stringset.
+
+Definition proj_mem (m: mem) (l: locs): mem :=
+  (filter (fun k => k ∈ l) m).
+
+Definition proj_env (e: env) (v: vars): env :=
+  (filter (fun k => k ∈ v) e).
+
+Definition proj (s: state) (v: vars) (l: locs)  :=
+  let (m, e) := s in
+  (proj_env e l, proj_mem m v).
+
+
+Definition upsilon (expr: expr) (state: state) : vars*locs :=
+let (mem, env) := state in
+match expr with
+| Const _ => (∅, ∅)
+| Addr x => match env !! x with
+           | Some l => ({[x]}, {[l]})
+           | None => (∅, ∅)
+           end
+| Deref e => match e with
+  | Addr x => match env !! x with
+              | Some l => ({[x]}, {[l]})
+              | None => (∅, ∅)
+              end
+  | _ => (∅, ∅)
+  end
+end.
+
+Definition upsilon_vars (expr: expr) (env: env): vars :=
+match expr with
+| Const _ => ∅
+| Addr x => match env !! x with
+           | Some l => {[x]}
+           | None => ∅
+           end
+| Deref e => match e with
+  | Addr x => match env !! x with
+              | Some l => {[x]}
+              | None => ∅
+              end
+  | _ => ∅
+  end
+end.
+
+Definition read (stmt: stmt) (state: state) : vars*locs :=
+  let (m, e) := state in
+  match stmt with
+  | Skip => (∅, ∅)
+  | Assign x expr => upsilon expr state
+  end.
+
+Definition read_vars (stmt: stmt) (env: env) : vars :=
+  match stmt with
+  | Skip => ∅
+  | Assign x expr => upsilon_vars expr env
+  end.
+
+Definition write (stmt: stmt) (state: state) : vars*locs :=
+  let (m, e) := state in
+  match stmt with
+  | Skip => (∅, ∅)
+  | Assign x expr => match e !! x with
+                    | Some l => ({[x]}, {[l]})
+                    | None => (∅, ∅)
+                    end
+  end.
+
+Definition write_vars (stmt: stmt) (env: env) : vars :=
+  match stmt with
+  | Skip => ∅
+  | Assign x expr => match env !! x with
+                    | Some l => {[x]}
+                    | None => ∅
+                    end
+  end.
+
+Theorem proj_env_eq: forall (e1 e2: env) (v: vars),
+  proj_env e1 v = proj_env e2 v -> forall (x: string), x ∈ v -> e1 !! x = e2 !! x.
+Proof.
+Admitted.
+
+Theorem proj_env_empty: forall (e: env),
+  proj_env e ∅ = ∅.
+Proof.
+  intros. unfold proj_env. 
+Admitted.
+
+Theorem proj_env_same: forall (m: mem) (e1 e2: env) (stmt: stmt) (r1 r2: vars),
+  r2 = read_vars stmt e2 /\
+  r1 = read_vars stmt e1 /\
+  r1 = r2 /\
+  proj_env e1 r1 = proj_env e2 r2  
+    -> proj_env (snd(eval_stmt m e1 stmt)) (write_vars stmt e1) = proj_env (snd(eval_stmt m e2 stmt)) (write_vars stmt e2).
+Proof.
+  intros. destruct H. destruct H0. destruct H1. destruct stmt0.
+  - simpl. simpl in H. simpl in H0. rewrite -> H0 in H2. rewrite -> H in H2. assumption.
+  - simpl in H. simpl in H0. destruct e.
+    + simpl. destruct (e2 !! x) eqn:He2x.
+      * destruct (e1 !! x) eqn:He1x.
+        -- simpl in H2.
+Abort.
