semantics/TotalMap.v
@@ -1,0 +1,98 @@
+From Coq Require Import Arith.Arith.
+From Coq Require Import Bool.Bool.
+Require Export Coq.Strings.String.
+From Coq Require Import Logic.FunctionalExtensionality.
+From Coq Require Import Lists.List.
+Import ListNotations.
+Set Default Goal Selector "!".
+
+Definition total_map (A:Type) := string -> A.
+
+Definition t_empty {A : Type} (v: A) : total_map A :=
+    (fun _ => v).
+
+Definition t_update {A: Type} (m: total_map A) (x: string) (v : A) :=
+    fun x' => if String.eqb x x' then v else m x'.
+
+Definition examplemap :=
+    t_update (t_update (t_empty false) "foo" true) "bar" true.
+
+Notation "'_' '!->' v" := (t_empty v)
+    (at level 100, right associativity).
+
+Example example_empty := (_ !-> false).
+
+Notation "x  '!->' v ';' m" := (t_update m x v)
+    (at level 100, v at next level, right associativity).
+
+Definition examplemap' := 
+    ( "bar" !-> true;
+      "foo" !-> true;
+       _ !-> false).
+
+Lemma t_apply_empty : forall (A: Type) (x : string) (v : A),
+    (_ !-> v) x = v.
+Proof.
+    intros. unfold t_empty. reflexivity.
+Qed.
+
+Lemma t_update_eq : forall (A : Type) (m: total_map A) x v,
+    (x !-> v; m) x = v.
+Proof.
+    intros. unfold t_update. rewrite eqb_refl. reflexivity.
+Qed.
+
+Lemma t_update_neq : forall (A : Type) (m: total_map A) x1 x2 v,
+    x1 <> x2 ->
+    (x1 !-> v; m) x2 = m x2.
+Proof.
+    intros. unfold t_update. rewrite <- eqb_neq in H. rewrite H. reflexivity.
+Qed.
+
+Lemma t_update_shadow : forall (A : Type) (m: total_map A) v1 v2 x,
+    (x !-> v2; x !-> v1; m) = (x !-> v2; m).
+Proof.
+    intros. unfold t_update. apply functional_extensionality. intros. destruct (eqb x x0) eqn:E.
+    - reflexivity.
+    - reflexivity.
+Qed.
+
+Lemma t_update_same : forall (A : Type) (m: total_map A) x,
+    (x !-> m x; m) = m.
+Proof.
+    intros. unfold t_update. apply functional_extensionality. intros. destruct (eqb_spec x x0).
+    - subst. reflexivity.
+    - reflexivity.
+Qed.
+
+
+Definition partial_map (A: Type) := total_map (option A).
+
+Definition empty {A: Type} : partial_map A := 
+    t_empty None.
+
+Definition update {A: Type} (m: partial_map A) (x: string) (v: A) :=
+    (x !-> (Some v); m).
+
+Notation "x '|->' v ';' m" := (update m x v)
+    (at level 100, v at next level, right associativity).
+
+Notation "x '|->' v" := (update empty x v)
+    (at level 100).
+
+Example example_partial_map :=
+    ("Church" |-> true; "Turing" |-> false).
+
+Lemma apply_empty : forall (A: Type) (x: string),
+    @empty A x = None.
+Proof.
+    intros. unfold empty. unfold t_empty. reflexivity. Qed.
+
+Lemma update_eq : forall (A: Type) (m: partial_map A) x v,
+    (x |-> v; m) x = Some v.
+Proof.
+    intros. unfold update. unfold t_update. rewrite eqb_refl. reflexivity.
+Qed.
+
+Definition includein {A: Type} (m m': partial_map A) :=
+    forall x v, m x = Some v -> m' x = Some v.
